src/Std/Data/DHashMap/Internal/Model.lean
@@ -322,6 +322,12 @@ def mapₘ (m : Raw₀ α β) (f : (a : α) → β a → δ a) : Raw₀ α δ :=
 def filterₘ (m : Raw₀ α β) (f : (a : α) → β a → Bool) : Raw₀ α β :=
   ⟨withComputedSize (updateAllBuckets m.1.buckets fun l => l.filter f), by simpa using m.2⟩
 
+/-- Internal implementation detail of the hash map -/
+def insertManyListₘ [BEq α] [Hashable α](m : Raw₀ α β) (l: List ((a : α) × β a)): Raw₀ α β :=
+  match l with
+  | .nil => m
+  | .cons hd tl => insertManyListₘ (m.insert hd.1 hd.2) tl
+
 section
 
 variable {β : Type v}
@@ -454,6 +460,14 @@ theorem map_eq_mapₘ (m : Raw₀ α β) (f : (a : α) → β a → δ a) :
 
 theorem filter_eq_filterₘ (m : Raw₀ α β) (f : (a : α) → β a → Bool) :
     m.filter f = m.filterₘ f := rfl
+
+theorem insertManyList_eq_insertManyListₘ [BEq α] [Hashable α](m : Raw₀ α β) (l: List ((a : α) × β a)): insertManyList m l = insertManyListₘ m l := by
+  simp [insertManyList, Id.run]
+  induction l generalizing m with
+  | nil => simp[insertManyListₘ]
+  | cons hd tl ih =>
+    simp [insertManyListₘ]
+    rw [ih]
 
 section
 
